reflection: TermEq: tidying up

ulib/FStar.Reflection.TermEq.fst
@@ -5,6 +5,11 @@ open FStar.Reflection.Data
 open FStar.Reflection.Builtins
 module L = FStar.List.Tot
 
+
+(* "SMT may not be able to prove the types of ... and ... to be equal,
+if the proof fails, try annotating these with the same type" *)
+#set-options "--warn_error -290"
+
 (*
 This file raised several limitations of the SMT encoding. Lines marked
 with #2908 are seemingly consequences of issue #2908 and should be removed.
@@ -59,6 +64,11 @@ let rec memP_dec #a (x : a) (l : list a)
     | y::ys ->
       if StrongExcludedMiddle.strong_excluded_middle (x == y) then () else memP_dec x ys
 
+(* FIXME: the only reason these are not exposed is to not contaminate
+the namespace for most users, especially as `Eq` is already used in
+Reflection.Formula. But there should not be a problem with using this
+name fully-qualified. *)
+private
 type _cmpres =
   | Eq
   | Neq
@@ -73,6 +83,7 @@ let valid #t (c:_cmpres) (x y : t) =
 
 type cmpres #t (x y : t) = c:_cmpres{valid c x y}
 
+unfold // FIXME: Only needed due to #2894
 type comparator_for (t:Type) = x:t -> y:t -> cmpres x y
 
 let (&&&) (#s : Type u#ss) (#t : Type u#tt) (#x #y : s) (#w #z : t)
@@ -85,138 +96,138 @@ let (&&&) (#s : Type u#ss) (#t : Type u#tt) (#x #y : s) (#w #z : t)
   | _, Neq -> Neq
   | _ -> Unknown
 
-val bv_eq : comparator_for bv
-let bv_eq x1 x2 =
+val bv_cmp : comparator_for bv
+let bv_cmp x1 x2 =
   let v1 = inspect_bv x1 in
   let v2 = inspect_bv x2 in
   pack_inspect_bv x1;
   pack_inspect_bv x2;
   if v1.bv_index = v2.bv_index then Eq else Neq
 
-val fv_eq : comparator_for fv
-let fv_eq f1 f2 =
+val fv_cmp : comparator_for fv
+let fv_cmp f1 f2 =
     pack_inspect_fv f1;
     pack_inspect_fv f2;
     let n1 = inspect_fv f1 in
     let n2 = inspect_fv f2 in
     if n1 = n2 then Eq else Neq
 
-val opt_eq : #a:Type -> comparator_for a -> comparator_for (option a)
-let opt_eq cmp o1 o2 =
+val opt_cmp : #a:Type -> comparator_for a -> comparator_for (option a)
+let opt_cmp cmp o1 o2 =
   match o1, o2 with
   | None, None -> Eq
   | Some x, Some y -> cmp x y
   | _ -> Neq
 
-val either_eq : #a:Type -> #b:Type -> comparator_for a -> comparator_for b -> comparator_for (either a b)
-let either_eq cmpa cmpb e1 e2 =
+val either_cmp : #a:Type -> #b:Type -> comparator_for a -> comparator_for b -> comparator_for (either a b)
+let either_cmp cmpa cmpb e1 e2 =
   match e1, e2 with
   | Inl x, Inl y -> cmpa x y
   | Inr x, Inr y -> cmpb x y
   | _ -> Neq
 
-val pair_eq : #a:Type -> #b:Type -> comparator_for a -> comparator_for b -> comparator_for (a & b)
-let pair_eq cmpa cmpb (a1, b1) (a2, b2) =
+val pair_cmp : #a:Type -> #b:Type -> comparator_for a -> comparator_for b -> comparator_for (a & b)
+let pair_cmp cmpa cmpb (a1, b1) (a2, b2) =
   cmpa a1 a2 &&& cmpb b1 b2
 
-val list_eq : #a:Type u#aa -> comparator_for a -> comparator_for (list a)
-let rec list_eq #a cmp l1 l2 =
+val list_cmp : #a:Type u#aa -> comparator_for a -> comparator_for (list a)
+let rec list_cmp #a cmp l1 l2 =
   match l1, l2 with
   | [], [] -> Eq
-  | x::xs, y::ys -> cmp x y &&& list_eq cmp xs ys
+  | x::xs, y::ys -> cmp x y &&& list_cmp cmp xs ys
   | _ -> Neq
 
-val list_dec_eq :
+val list_dec_cmp :
 #a:Type u#aa -> #b:Type u#bb -> top1:b -> top2:b ->
   f:(x:a -> y:a{x << top1 /\ y << top2} -> cmpres x y) ->
   l1:(list a) -> l2:(list a){l1 << top1 /\ l2 << top2} ->
   cmpres l1 l2
-let rec list_dec_eq #a top1 top2 cmp l1 l2 =
+let rec list_dec_cmp #a top1 top2 cmp l1 l2 =
   match l1, l2 with
   | [], [] -> Eq
-  | x::xs, y::ys -> cmp x y &&& list_dec_eq top1 top2 cmp xs ys
+  | x::xs, y::ys -> cmp x y &&& list_dec_cmp top1 top2 cmp xs ys
   | _ -> Neq
 
-val opt_dec_eq : #a:Type -> #b:Type -> top1:b -> top2:b ->
+val opt_dec_cmp : #a:Type -> #b:Type -> top1:b -> top2:b ->
   (f : (x:a -> y:a{x << top1 /\ y << top2} -> cmpres x y)) ->
   o1:(option a){o1 << top1} -> o2:(option a){o2 << top2} ->
   cmpres o1 o2
-let opt_dec_eq top1 top2 cmp o1 o2 =
+let opt_dec_cmp top1 top2 cmp o1 o2 =
   match o1, o2 with
   | None, None -> Eq
   | Some x, Some y -> cmp x y
   | _ -> Neq
 
-val either_dec_eq : #a:Type -> #b:Type -> #c:Type -> top1:c -> top2:c ->
+val either_dec_cmp : #a:Type -> #b:Type -> #c:Type -> top1:c -> top2:c ->
   (x:a -> y:a{x<<top1 /\ y<<top2} -> cmpres x y) ->
   (x:b -> y:b{x<<top1 /\ y<<top2} -> cmpres x y) ->
   e1 :(either a b){e1 << top1} ->
   e2 :(either a b){e2 << top2} ->
   cmpres e1 e2
-let either_dec_eq top1 top2 cmpa cmpb e1 e2 =
+let either_dec_cmp top1 top2 cmpa cmpb e1 e2 =
   match e1, e2 with
   | Inl x, Inl y -> cmpa x y
   | Inr x, Inr y -> cmpb x y
   | _ -> Neq
 
-val eq_eq : #a:eqtype -> comparator_for a
-let eq_eq x y = if x = y then Eq else Neq
+val eq_cmp : #a:eqtype -> comparator_for a
+let eq_cmp x y = if x = y then Eq else Neq
 
-val range_eq : comparator_for range
-let range_eq r1 r2 =
+val range_cmp : comparator_for range
+let range_cmp r1 r2 =
   Sealed.sealed_singl r1 r2;
   Eq
 
-val ident_eq : comparator_for ident
-let ident_eq i1 i2 =
+val ident_cmp : comparator_for ident
+let ident_cmp i1 i2 =
   Sealed.sealed_singl (snd i1) (snd i2);
-  eq_eq (fst i1) (fst i2)
+  eq_cmp (fst i1) (fst i2)
 
-val univ_eq : comparator_for universe
-let rec univ_eq (u1 u2 : universe) =
+val univ_cmp : comparator_for universe
+let rec univ_cmp (u1 u2 : universe) =
   pack_inspect_universe u1;
   pack_inspect_universe u2;
   let uv1 = inspect_universe u1 in
   let uv2 = inspect_universe u2 in
   match uv1, uv2 with
   | Uv_Zero, Uv_Zero -> Eq
-  | Uv_Succ u1, Uv_Succ u2 -> univ_eq u1 u2
-  | Uv_Max us1, Uv_Max us2 -> list_dec_eq u1 u2 univ_eq us1 us2
-  | Uv_BVar v1, Uv_BVar v2 -> eq_eq v1 v2
-  | Uv_Name n1, Uv_Name n2 -> ident_eq n1 n2
+  | Uv_Succ u1, Uv_Succ u2 -> univ_cmp u1 u2
+  | Uv_Max us1, Uv_Max us2 -> list_dec_cmp u1 u2 univ_cmp us1 us2
+  | Uv_BVar v1, Uv_BVar v2 -> eq_cmp v1 v2
+  | Uv_Name n1, Uv_Name n2 -> ident_cmp n1 n2
   | Uv_Unif u1, Uv_Unif u2 -> Unknown
   | Uv_Unk, Uv_Unk -> Eq
   | _ -> Neq
 
-val const_eq : comparator_for vconst
-let const_eq c1 c2 =
+val const_cmp : comparator_for vconst
+let const_cmp c1 c2 =
   match c1, c2 with
   | C_Unit, C_Unit -> Eq
-  | C_Int i1, C_Int i2 -> eq_eq i1 i2
+  | C_Int i1, C_Int i2 -> eq_cmp i1 i2
   | C_True, C_True -> Eq
   | C_False, C_False -> Eq
-  | C_String s1, C_String s2 -> eq_eq s1 s2
-  | C_Range r1, C_Range r2 -> range_eq r1 r2
+  | C_String s1, C_String s2 -> eq_cmp s1 s2
+  | C_Range r1, C_Range r2 -> range_cmp r1 r2
   | C_Reify, C_Reify -> Eq
-  | C_Reflect n1, C_Reflect n2 -> eq_eq n1 n2
+  | C_Reflect n1, C_Reflect n2 -> eq_cmp n1 n2
   | _ -> Neq
 
 (* TODO. Or seal...? *)
-val ctxu_eq : comparator_for ctx_uvar_and_subst
-let ctxu_eq _ _ = Unknown
+val ctxu_cmp : comparator_for ctx_uvar_and_subst
+let ctxu_cmp _ _ = Unknown
 
-val term_eq         : comparator_for term
-val binder_eq       : comparator_for binder
-val aqual_eq        : comparator_for aqualv
-val arg_eq          : comparator_for argv
-val binding_bv_eq   : comparator_for bv
-val comp_eq         : comparator_for comp
-val pat_eq          : comparator_for pattern
-val pat_arg_eq      : comparator_for (pattern & bool)
-val br_eq           : comparator_for branch
-val match_returns_ascription_eq : comparator_for match_returns_ascription
+val term_cmp         : comparator_for term
+val binder_cmp       : comparator_for binder
+val aqual_cmp        : comparator_for aqualv
+val arg_cmp          : comparator_for argv
+val binding_bv_cmp   : comparator_for bv
+val comp_cmp         : comparator_for comp
+val pat_cmp          : comparator_for pattern
+val pat_arg_cmp      : comparator_for (pattern & bool)
+val br_cmp           : comparator_for branch
+val match_returns_ascription_cmp : comparator_for match_returns_ascription
 
-let rec term_eq t1 t2 =
+let rec term_cmp t1 t2 =
   pack_inspect_inv t1;
   pack_inspect_inv t2;
   let tv1 = inspect_ln t1 in
@@ -224,77 +235,79 @@ let rec term_eq t1 t2 =
   match tv1, tv2 with
   | Tv_Unsupp, _
   | _, Tv_Unsupp -> Unknown
-  | Tv_Var v1, Tv_Var v2 -> bv_eq v1 v2
-  | Tv_BVar v1, Tv_BVar v2 -> bv_eq v1 v2
-  | Tv_FVar f1, Tv_FVar f2 -> fv_eq f1 f2
+  | Tv_Var v1, Tv_Var v2 -> bv_cmp v1 v2
+  | Tv_BVar v1, Tv_BVar v2 -> bv_cmp v1 v2
+  | Tv_FVar f1, Tv_FVar f2 -> fv_cmp f1 f2
   | Tv_UInst f1 u1, Tv_UInst f2 u2 ->
-    fv_eq f1 f2 &&& list_dec_eq t1 t2 univ_eq u1 u2
+    fv_cmp f1 f2 &&& list_dec_cmp t1 t2 univ_cmp u1 u2
 
   | Tv_App h1 a1, Tv_App h2 a2 ->
-    term_eq h1 h2 &&& arg_eq a1 a2
+    term_cmp h1 h2 &&& arg_cmp a1 a2
 
   | Tv_Abs b1 e1, Tv_Abs b2 e2 ->
-    binder_eq b1 b2
-     &&& term_eq e1 e2
+    binder_cmp b1 b2
+     &&& term_cmp e1 e2
 
   | Tv_Arrow b1 c1, Tv_Arrow b2 c2 ->
-    binder_eq b1 b2
-     &&& comp_eq c1 c2
+    binder_cmp b1 b2
+     &&& comp_cmp c1 c2
 
   | Tv_Type u1, Tv_Type u2 ->
-    univ_eq u1 u2
+    univ_cmp u1 u2
 
   | Tv_Refine v1 sort1 r1, Tv_Refine v2 sort2 r2 ->
-    binding_bv_eq v1 v2
-     &&& term_eq sort1 sort2
-     &&& term_eq r1 r2
+    binding_bv_cmp v1 v2
+     &&& term_cmp sort1 sort2
+     &&& term_cmp r1 r2
 
   | Tv_Const c1, Tv_Const c2 ->
-    const_eq c1 c2
+    const_cmp c1 c2
 
   | Tv_Uvar n1 u1, Tv_Uvar n2 u2 ->
-    eq_eq n1 n2 &&& ctxu_eq u1 u2
+    eq_cmp n1 n2 &&& ctxu_cmp u1 u2
 
   | Tv_Let r1 attrs1 bv1 ty1 e1 b1, Tv_Let r2 attrs2 bv2 ty2 e2 b2 ->
-    eq_eq r1 r2
-     &&& list_dec_eq t1 t2 term_eq attrs1 attrs2
-     &&& binding_bv_eq bv1 bv2
-     &&& term_eq ty1 ty2
-     &&& term_eq e1 e2
-     &&& term_eq b1 b2
+    eq_cmp r1 r2
+     &&& list_dec_cmp t1 t2 term_cmp attrs1 attrs2
+     &&& binding_bv_cmp bv1 bv2
+     &&& term_cmp ty1 ty2
+     &&& term_cmp e1 e2
+     &&& term_cmp b1 b2
 
   | Tv_Match sc1 o1 brs1, Tv_Match sc2 o2 brs2 ->
-    term_eq sc1 sc2
-     &&& opt_dec_eq t1 t2 match_returns_ascription_eq o1 o2
-     &&& list_dec_eq t1 t2 br_eq brs1 brs2
+    term_cmp sc1 sc2
+     &&& opt_dec_cmp t1 t2 match_returns_ascription_cmp o1 o2
+     &&& list_dec_cmp t1 t2 br_cmp brs1 brs2
 
   | Tv_AscribedT e1 ta1 tacopt1 eq1, Tv_AscribedT e2 ta2 tacopt2 eq2 ->
-    term_eq e1 e2
-     &&& term_eq ta1 ta2
-     &&& opt_dec_eq t1 t2 term_eq tacopt1 tacopt2
-     &&& eq_eq eq1 eq2
+    term_cmp e1 e2
+     &&& term_cmp ta1 ta2
+     &&& opt_dec_cmp t1 t2 term_cmp tacopt1 tacopt2
+     &&& eq_cmp eq1 eq2
 
   | Tv_AscribedC e1 c1 tacopt1 eq1, Tv_AscribedC e2 c2 tacopt2 eq2 ->
-    term_eq e1 e2
-     &&& comp_eq c1 c2
-     &&& opt_dec_eq t1 t2 term_eq tacopt1 tacopt2
-     &&& eq_eq eq1 eq2
+    term_cmp e1 e2
+     &&& comp_cmp c1 c2
+     &&& opt_dec_cmp t1 t2 term_cmp tacopt1 tacopt2
+     &&& eq_cmp eq1 eq2
 
   | Tv_Unknown, Tv_Unknown -> Eq
 
   | _ -> Neq
 
-and arg_eq (a1, q1) (a2, q2) =
-  term_eq a1 a2 &&& aqual_eq q1 q2
+and arg_cmp (a1, q1) (a2, q2) =
+  term_cmp a1 a2 &&& aqual_cmp q1 q2
 
-and aqual_eq a1 a2 =
+and aqual_cmp a1 a2 =
   match a1, a2 with
   | Q_Implicit, Q_Implicit -> Eq
   | Q_Explicit, Q_Explicit -> Eq
-  | Q_Meta m1, Q_Meta m2 -> term_eq m1 m2
+  | Q_Meta m1, Q_Meta m2 -> term_cmp m1 m2
   | _ -> Neq
 
-and binding_bv_eq x1 x2 =
+(* FIXME: currently we need to compare the indices
+of binding bvs, but they should not matter at all. *)
+and binding_bv_cmp x1 x2 =
   let v1 = inspect_bv x1 in
   let v2 = inspect_bv x2 in
   pack_inspect_bv x1;
@@ -303,25 +316,25 @@ and binding_bv_eq x1 x2 =
    then Eq
    else Neq
 
-and match_returns_ascription_eq asc1 asc2 =
+and match_returns_ascription_cmp asc1 asc2 =
   let (b1, (tc1, tacopt1, eq1)) = asc1 in
   let (b2, (tc2, tacopt2, eq2)) = asc2 in
-  binder_eq b1 b2
-   &&& either_dec_eq asc1 asc2 term_eq comp_eq tc1 tc2
-   &&& opt_dec_eq asc1 asc2 term_eq tacopt1 tacopt2
-   &&& eq_eq eq1 eq2
+  binder_cmp b1 b2
+   &&& either_dec_cmp asc1 asc2 term_cmp comp_cmp tc1 tc2
+   &&& opt_dec_cmp asc1 asc2 term_cmp tacopt1 tacopt2
+   &&& eq_cmp eq1 eq2
 
-and binder_eq b1 b2 =
+and binder_cmp b1 b2 =
   let bv1 = inspect_binder b1 in
   let bv2 = inspect_binder b2 in
   pack_inspect_binder b1;
   pack_inspect_binder b2;
-  binding_bv_eq bv1.binder_bv bv2.binder_bv
-   &&& term_eq bv1.binder_sort bv2.binder_sort
-   &&& aqual_eq bv1.binder_qual bv2.binder_qual
-   &&& list_dec_eq b1 b2 term_eq bv1.binder_attrs bv2.binder_attrs
+  binding_bv_cmp bv1.binder_bv bv2.binder_bv
+   &&& term_cmp bv1.binder_sort bv2.binder_sort
+   &&& aqual_cmp bv1.binder_qual bv2.binder_qual
+   &&& list_dec_cmp b1 b2 term_cmp bv1.binder_attrs bv2.binder_attrs
 
-and comp_eq c1 c2 =
+and comp_cmp c1 c2 =
   let cv1 = inspect_comp c1 in
   let cv2 = inspect_comp c2 in
   pack_inspect_comp_inv c1;
@@ -329,49 +342,49 @@ and comp_eq c1 c2 =
   match cv1, cv2 with
   | C_Total t1, C_Total t2
   | C_GTotal t1, C_GTotal t2 ->
-    term_eq t1 t2
+    term_cmp t1 t2
 
   | C_Lemma pre1 post1 pat1, C_Lemma pre2 post2 pat2 ->
-    term_eq pre1 pre2
-     &&& term_eq post1 post2
-     &&& term_eq pat1 pat2
+    term_cmp pre1 pre2
+     &&& term_cmp post1 post2
+     &&& term_cmp pat1 pat2
 
   | C_Eff us1 ef1 t1 args1 dec1, C_Eff us2 ef2 t2 args2 dec2 ->
-    list_dec_eq c1 c2 univ_eq us1 us2
-     &&& eq_eq ef1 ef2
-     &&& term_eq t1 t2
-     &&& list_dec_eq c1 c2 arg_eq args1 args2
-     &&& list_dec_eq c1 c2 term_eq dec1 dec2
+    list_dec_cmp c1 c2 univ_cmp us1 us2
+     &&& eq_cmp ef1 ef2
+     &&& term_cmp t1 t2
+     &&& list_dec_cmp c1 c2 arg_cmp args1 args2
+     &&& list_dec_cmp c1 c2 term_cmp dec1 dec2
 
   | _ -> Neq
 
-and br_eq br1 br2 =
-  //pair_eq pat_eq term_eq br1 br2
-  pat_eq (fst br1) (fst br2) &&& term_eq (snd br1) (snd br2)
+and br_cmp br1 br2 =
+  //pair_cmp pat_cmp term_cmp br1 br2
+  pat_cmp (fst br1) (fst br2) &&& term_cmp (snd br1) (snd br2)
 
-and pat_eq p1 p2 =
+and pat_cmp p1 p2 =
   match p1, p2 with
   | Pat_Var v1 st1, Pat_Var v2 st2 ->
     Sealed.sealed_singl st1 st2;
-    bv_eq v1 v2
-  | Pat_Constant c1, Pat_Constant c2 -> const_eq c1 c2
-  | Pat_Dot_Term t1, Pat_Dot_Term t2 -> opt_dec_eq p1 p2 term_eq t1 t2
+    bv_cmp v1 v2
+  | Pat_Constant c1, Pat_Constant c2 -> const_cmp c1 c2
+  | Pat_Dot_Term t1, Pat_Dot_Term t2 -> opt_dec_cmp p1 p2 term_cmp t1 t2
   | Pat_Cons f1 us1 args1, Pat_Cons f2 us2 args2 ->
-    fv_eq f1 f2
-     &&& opt_dec_eq p1 p2 (list_dec_eq p1 p2 univ_eq) us1 us2
-     &&& list_dec_eq p1 p2 pat_arg_eq args1 args2
+    fv_cmp f1 f2
+     &&& opt_dec_cmp p1 p2 (list_dec_cmp p1 p2 univ_cmp) us1 us2
+     &&& list_dec_cmp p1 p2 pat_arg_cmp args1 args2
 
   | _ -> Neq
 
-and pat_arg_eq (p1, b1) (p2, b2) =
-  pat_eq p1 p2 &&& eq_eq b1 b2
+and pat_arg_cmp (p1, b1) (p2, b2) =
+  pat_cmp p1 p2 &&& eq_cmp b1 b2
 
 let defined r = ~(Unknown? r)
 
 let def2 f l1 l2 =(forall x y. L.memP x l1 /\ L.memP y l2 ==> defined (f x y))
 
 let rec defined_list #a (f : comparator_for a) (l1 l2 : list a)
-  : Lemma (requires (def2 f l1 l2)) (ensures defined (list_eq f l1 l2))
+  : Lemma (requires (def2 f l1 l2)) (ensures defined (list_cmp f l1 l2))
   = match l1, l2 with
     | [], [] -> ()
     | x::xs, y::ys -> defined_list f xs ys
@@ -380,7 +393,7 @@ let rec defined_list #a (f : comparator_for a) (l1 l2 : list a)
 let rec defined_list_dec #a #b (t1 t2 : b) (f : comparator_for a)
   (l1 : list a{l1 << t1})
   (l2 : list a{l2 << t2})
-  : Lemma (requires (def2 f l1 l2)) (ensures defined (list_dec_eq t1 t2 f l1 l2))
+  : Lemma (requires (def2 f l1 l2)) (ensures defined (list_dec_cmp t1 t2 f l1 l2))
   = match l1, l2 with
     | [], [] -> ()
     | x::xs, y::ys -> defined_list_dec t1 t2 f xs ys
@@ -407,10 +420,10 @@ let faithful_univ_UvMax (u : universe) (us : list universe)
 let univ_eq_UvMax (u1 u2 : universe) (us1 us2 : list universe)
   : Lemma (requires inspect_universe u1 == Uv_Max us1 /\
                     inspect_universe u2 == Uv_Max us2)
-          (ensures univ_eq u1 u2 == list_dec_eq u1 u2 univ_eq us1 us2)
-  = assert_norm (univ_eq u1 u2 == list_dec_eq u1 u2 univ_eq us1 us2) // #2908
+          (ensures univ_cmp u1 u2 == list_dec_cmp u1 u2 univ_cmp us1 us2)
+  = assert_norm (univ_cmp u1 u2 == list_dec_cmp u1 u2 univ_cmp us1 us2) // #2908
 
-val univ_faithful_lemma (u1 u2 : universe) : Lemma (requires faithful_univ u1 /\ faithful_univ u2) (ensures defined (univ_eq u1 u2))
+val univ_faithful_lemma (u1 u2 : universe) : Lemma (requires faithful_univ u1 /\ faithful_univ u2) (ensures defined (univ_cmp u1 u2))
 let rec univ_faithful_lemma (u1 u2 : universe) =
   match inspect_universe u1, inspect_universe u2 with
   | Uv_Zero, Uv_Zero -> ()
@@ -427,18 +440,18 @@ let rec univ_faithful_lemma (u1 u2 : universe) =
 
 and univ_faithful_lemma_list #b (u1 u2 : b) (us1 : list universe{us1 << u1}) (us2 : list universe{us2 << u2})
   : Lemma (requires allP u1 faithful_univ us1 /\ allP u2 faithful_univ us2)
-          (ensures defined (list_dec_eq u1 u2 univ_eq us1 us2))
+          (ensures defined (list_dec_cmp u1 u2 univ_cmp us1 us2))
           (decreases us1)
   =
-    introduce forall x y. L.memP x us1 /\ L.memP y us2 ==> defined (univ_eq x y) with
-     (introduce forall y. L.memP x us1 /\ L.memP y us2 ==> defined (univ_eq x y) with
-      (introduce (L.memP x us1 /\ L.memP y us2) ==> (defined (univ_eq x y)) with h. (
+    introduce forall x y. L.memP x us1 /\ L.memP y us2 ==> defined (univ_cmp x y) with
+     (introduce forall y. L.memP x us1 /\ L.memP y us2 ==> defined (univ_cmp x y) with
+      (introduce (L.memP x us1 /\ L.memP y us2) ==> (defined (univ_cmp x y)) with h. (
        univ_faithful_lemma x y
        )
       )
      )
     ;
-    defined_list_dec u1 u2 univ_eq us1 us2
+    defined_list_dec u1 u2 univ_cmp us1 us2
 
 val faithful : term -> Type0
 let rec faithful t =
@@ -533,7 +546,7 @@ and faithful_comp c =
      /\ allP c faithful_arg args
      /\ allP c faithful decs
 
-val faithful_lemma (t1:term) (t2:term) : Lemma (requires faithful t1 /\ faithful t2) (ensures defined (term_eq t1 t2))
+val faithful_lemma (t1:term) (t2:term) : Lemma (requires faithful t1 /\ faithful t2) (ensures defined (term_cmp t1 t2))
 
 #push-options "--z3rlimit 40"
 
@@ -552,8 +565,8 @@ let faithful_Tv_Let (t : term) (recf : bool) (attrs : list term) (bv:bv) (ty:typ
 let term_eq_Tv_Let (t1 t2 : term) (recf1 recf2 : bool) (attrs1 attrs2 : list term) (bv1 bv2:bv) (ty1 ty2:typ) (def1 def2 body1 body2: term)
   : Lemma (requires inspect_ln t1 == Tv_Let recf1 attrs1 bv1 ty1 def1 body1
                   /\ inspect_ln t2 == Tv_Let recf2 attrs2 bv2 ty2 def2 body2)
-          (ensures term_eq t1 t2 == (eq_eq recf1 recf2 &&& list_dec_eq t1 t2 term_eq attrs1 attrs2 &&& binding_bv_eq bv1 bv2 &&& term_eq ty1 ty2 &&& term_eq def1 def2 &&& term_eq body1 body2))
-  = assume (term_eq t1 t2 == (eq_eq recf1 recf2 &&& list_dec_eq t1 t2 term_eq attrs1 attrs2 &&& binding_bv_eq bv1 bv2 &&& term_eq ty1 ty2 &&& term_eq def1 def2 &&& term_eq body1 body2)) // #2908, somehow assert_norm also does not work
+          (ensures term_cmp t1 t2 == (eq_cmp recf1 recf2 &&& list_dec_cmp t1 t2 term_cmp attrs1 attrs2 &&& binding_bv_cmp bv1 bv2 &&& term_cmp ty1 ty2 &&& term_cmp def1 def2 &&& term_cmp body1 body2))
+  = assume (term_cmp t1 t2 == (eq_cmp recf1 recf2 &&& list_dec_cmp t1 t2 term_cmp attrs1 attrs2 &&& binding_bv_cmp bv1 bv2 &&& term_cmp ty1 ty2 &&& term_cmp def1 def2 &&& term_cmp body1 body2)) // #2908, somehow assert_norm also does not work
 
 let faithful_Tv_Match (t : term) (sc : term) (o : option match_returns_ascription) (brs : list branch)
   : Lemma (requires inspect_ln t == Tv_Match sc o brs /\ faithful t)
@@ -563,12 +576,12 @@ let faithful_Tv_Match (t : term) (sc : term) (o : option match_returns_ascriptio
 let term_eq_Tv_Match (t1 t2 : term) (sc1 sc2 : term) (o1 o2 : option match_returns_ascription) (brs1 brs2 : list branch)
   : Lemma (requires inspect_ln t1 == Tv_Match sc1 o1 brs1
                   /\ inspect_ln t2 == Tv_Match sc2 o2 brs2)
-          (ensures term_eq t1 t2 == (term_eq sc1 sc2
-                    &&& opt_dec_eq t1 t2 match_returns_ascription_eq o1 o2
-                    &&& list_dec_eq t1 t2 br_eq brs1 brs2))
-  = assume (term_eq t1 t2 == (term_eq sc1 sc2
-                    &&& opt_dec_eq t1 t2 match_returns_ascription_eq o1 o2
-                   &&& list_dec_eq t1 t2 br_eq brs1 brs2)) // #2908, somehow assert_norm also does not work
+          (ensures term_cmp t1 t2 == (term_cmp sc1 sc2
+                    &&& opt_dec_cmp t1 t2 match_returns_ascription_cmp o1 o2
+                    &&& list_dec_cmp t1 t2 br_cmp brs1 brs2))
+  = assume (term_cmp t1 t2 == (term_cmp sc1 sc2
+                    &&& opt_dec_cmp t1 t2 match_returns_ascription_cmp o1 o2
+                   &&& list_dec_cmp t1 t2 br_cmp brs1 brs2)) // #2908, somehow assert_norm also does not work
 
 let faithful_Pat_Cons (p : pattern) (f:fv) (ous : option universes) (args : list (pattern & bool))
   : Lemma (requires p == Pat_Cons f ous args /\ faithful_pattern p)
@@ -577,26 +590,26 @@ let faithful_Pat_Cons (p : pattern) (f:fv) (ous : option universes) (args : list
 
 let pat_eq_Pat_Cons (p1 p2 : pattern) (f1 f2 : fv) (ous1 ous2 : option universes) (args1 args2 : list (pattern & bool))
   : Lemma (requires p1 == Pat_Cons f1 ous1 args1 /\ p2 == Pat_Cons f2 ous2 args2)
-          (ensures pat_eq p1 p2 == (fv_eq f1 f2
-                                    &&& opt_dec_eq p1 p2 (list_dec_eq p1 p2 univ_eq) ous1 ous2
-                                    &&& list_dec_eq p1 p2 pat_arg_eq args1 args2))
-  = assert_norm (pat_eq p1 p2 == (fv_eq f1 f2
-                                    &&& opt_dec_eq p1 p2 (list_dec_eq p1 p2 univ_eq) ous1 ous2
-                                    &&& list_dec_eq p1 p2 pat_arg_eq args1 args2))
+          (ensures pat_cmp p1 p2 == (fv_cmp f1 f2
+                                    &&& opt_dec_cmp p1 p2 (list_dec_cmp p1 p2 univ_cmp) ous1 ous2
+                                    &&& list_dec_cmp p1 p2 pat_arg_cmp args1 args2))
+  = assert_norm (pat_cmp p1 p2 == (fv_cmp f1 f2
+                                    &&& opt_dec_cmp p1 p2 (list_dec_cmp p1 p2 univ_cmp) ous1 ous2
+                                    &&& list_dec_cmp p1 p2 pat_arg_cmp args1 args2))
 
 let comp_eq_C_Eff (c1 c2 : comp) (us1 us2 : universes) (ef1 ef2 : name) (t1 t2 : typ) (args1 args2 : list argv) (dec1 dec2 : list term)
   : Lemma (requires inspect_comp c1 == C_Eff us1 ef1 t1 args1 dec1
                   /\ inspect_comp c2 == C_Eff us2 ef2 t2 args2 dec2)
-          (ensures comp_eq c1 c2 == (list_dec_eq c1 c2 univ_eq us1 us2
-                                        &&& eq_eq ef1 ef2
-                                        &&& term_eq t1 t2
-                                        &&& list_dec_eq c1 c2 arg_eq args1 args2
-                                        &&& list_dec_eq c1 c2 term_eq dec1 dec2))
-  = assume (comp_eq c1 c2 == (list_dec_eq c1 c2 univ_eq us1 us2
-                                        &&& eq_eq ef1 ef2
-                                        &&& term_eq t1 t2
-                                        &&& list_dec_eq c1 c2 arg_eq args1 args2
-                                        &&& list_dec_eq c1 c2 term_eq dec1 dec2)) // #2908, assert_norm doesn't work
+          (ensures comp_cmp c1 c2 == (list_dec_cmp c1 c2 univ_cmp us1 us2
+                                        &&& eq_cmp ef1 ef2
+                                        &&& term_cmp t1 t2
+                                        &&& list_dec_cmp c1 c2 arg_cmp args1 args2
+                                        &&& list_dec_cmp c1 c2 term_cmp dec1 dec2))
+  = assume (comp_cmp c1 c2 == (list_dec_cmp c1 c2 univ_cmp us1 us2
+                                        &&& eq_cmp ef1 ef2
+                                        &&& term_cmp t1 t2
+                                        &&& list_dec_cmp c1 c2 arg_cmp args1 args2
+                                        &&& list_dec_cmp c1 c2 term_cmp dec1 dec2)) // #2908, assert_norm doesn't work
 
 let rec faithful_lemma (t1 t2 : term) =
   match inspect_ln t1, inspect_ln t2 with
@@ -655,9 +668,9 @@ let rec faithful_lemma (t1 t2 : term) =
 
   | Tv_Unknown, Tv_Unknown -> ()
 
-  | _ -> assert (defined (term_eq t1 t2)) (* rest of the cases trivial *)
+  | _ -> assert (defined (term_cmp t1 t2)) (* rest of the cases trivial *)
 
-and faithful_lemma_pattern (p1 p2 : pattern) : Lemma (requires faithful_pattern p1 /\ faithful_pattern p2) (ensures defined (pat_eq p1 p2)) =
+and faithful_lemma_pattern (p1 p2 : pattern) : Lemma (requires faithful_pattern p1 /\ faithful_pattern p2) (ensures defined (pat_cmp p1 p2)) =
   match p1, p2 with
   | Pat_Var v1 _, Pat_Var v2 _ -> ()
   | Pat_Constant c1, Pat_Constant c2 -> ()
@@ -665,7 +678,7 @@ and faithful_lemma_pattern (p1 p2 : pattern) : Lemma (requires faithful_pattern 
   | Pat_Cons f1 uso1 args1, Pat_Cons f2 uso2 args2 ->
     (***)faithful_Pat_Cons p1 f1 uso1 args1;
     (***)faithful_Pat_Cons p2 f2 uso2 args2;
-    let aux : squash (defined (opt_dec_eq p1 p2 (list_dec_eq p1 p2 univ_eq) uso1 uso2)) =
+    let aux : squash (defined (opt_dec_cmp p1 p2 (list_dec_cmp p1 p2 univ_cmp) uso1 uso2)) =
       match uso1, uso2 with
       | Some us1, Some us2 ->
         univ_faithful_lemma_list p1 p2 us1 us2
@@ -678,7 +691,7 @@ and faithful_lemma_pattern (p1 p2 : pattern) : Lemma (requires faithful_pattern 
 
 and faithful_lemma_pattern_arg (pb1 pb2 : pattern & bool)
   : Lemma (requires faithful_pattern_arg pb1 /\ faithful_pattern_arg pb2)
-          (ensures defined (pat_arg_eq pb1 pb2))
+          (ensures defined (pat_arg_cmp pb1 pb2))
   =
   let (p1, _) = pb1 in
   let (p2, _) = pb2 in
@@ -689,20 +702,20 @@ and faithful_lemma_pattern_args #b
   (pats1 : list (pattern & bool){pats1 << top1})
   (pats2 : list (pattern & bool){pats2 << top2})
   : Lemma (requires allP top1 faithful_pattern_arg pats1 /\ allP top2 faithful_pattern_arg pats2)
-          (ensures defined (list_dec_eq top1 top2 pat_arg_eq pats1 pats2))
+          (ensures defined (list_dec_cmp top1 top2 pat_arg_cmp pats1 pats2))
           (decreases pats1)
   =
-  introduce forall x y. L.memP x pats1 /\ L.memP y pats2 ==> defined (pat_arg_eq x y) with
-   (introduce forall y. L.memP x pats1 /\ L.memP y pats2 ==> defined (pat_arg_eq x y) with
-    (introduce (L.memP x pats1 /\ L.memP y pats2) ==> (defined (pat_arg_eq x y)) with h. (
+  introduce forall x y. L.memP x pats1 /\ L.memP y pats2 ==> defined (pat_arg_cmp x y) with
+   (introduce forall y. L.memP x pats1 /\ L.memP y pats2 ==> defined (pat_arg_cmp x y) with
+    (introduce (L.memP x pats1 /\ L.memP y pats2) ==> (defined (pat_arg_cmp x y)) with h. (
      faithful_lemma_pattern_arg x y
      )
     )
    )
   ;
-  defined_list_dec top1 top2 pat_arg_eq pats1 pats2
+  defined_list_dec top1 top2 pat_arg_cmp pats1 pats2
 
-and faithful_lemma_branch (br1 br2 : branch) : Lemma (requires faithful_branch br1 /\ faithful_branch br2) (ensures defined (br_eq br1 br2)) =
+and faithful_lemma_branch (br1 br2 : branch) : Lemma (requires faithful_branch br1 /\ faithful_branch br2) (ensures defined (br_cmp br1 br2)) =
   faithful_lemma_pattern (fst br1) (fst br2);
   faithful_lemma (snd br1) (snd br2)
 
@@ -710,37 +723,37 @@ and faithful_lemma_branches #b (top1 top2 : b)
   (brs1 : list branch{brs1 << top1})
   (brs2 : list branch{brs2 << top2})
   : Lemma (requires allP top1 faithful_branch brs1 /\ allP top2 faithful_branch brs2)
-          (ensures defined (list_dec_eq top1 top2 br_eq brs1 brs2))
+          (ensures defined (list_dec_cmp top1 top2 br_cmp brs1 brs2))
           (decreases brs1)
   =
-  introduce forall x y. L.memP x brs1 /\ L.memP y brs2 ==> defined (br_eq x y) with
-   (introduce forall y. L.memP x brs1 /\ L.memP y brs2 ==> defined (br_eq x y) with
-    (introduce (L.memP x brs1 /\ L.memP y brs2) ==> (defined (br_eq x y)) with h. (
+  introduce forall x y. L.memP x brs1 /\ L.memP y brs2 ==> defined (br_cmp x y) with
+   (introduce forall y. L.memP x brs1 /\ L.memP y brs2 ==> defined (br_cmp x y) with
+    (introduce (L.memP x brs1 /\ L.memP y brs2) ==> (defined (br_cmp x y)) with h. (
      faithful_lemma_branch x y
      )
     )
    )
   ;
-  defined_list_dec top1 top2 br_eq brs1 brs2
+  defined_list_dec top1 top2 br_cmp brs1 brs2
 
-and faithful_lemma_arg (a1 a2 : argv) : Lemma (requires faithful_arg a1 /\ faithful_arg a2) (ensures defined (arg_eq a1 a2)) =
+and faithful_lemma_arg (a1 a2 : argv) : Lemma (requires faithful_arg a1 /\ faithful_arg a2) (ensures defined (arg_cmp a1 a2)) =
   faithful_lemma (fst a1) (fst a2);
   (match snd a1, snd a2 with | Q_Meta t1, Q_Meta t2 -> faithful_lemma t1 t2 | _ -> ())
 
-and faithful_lemma_binder (b1 b2 : binder) : Lemma (requires faithful_binder b1 /\ faithful_binder b2) (ensures defined (binder_eq b1 b2)) =
+and faithful_lemma_binder (b1 b2 : binder) : Lemma (requires faithful_binder b1 /\ faithful_binder b2) (ensures defined (binder_cmp b1 b2)) =
   let bv1 = inspect_binder b1 in
   let bv2 = inspect_binder b2 in
   faithful_lemma_qual bv1.binder_qual bv2.binder_qual;
   faithful_lemma bv1.binder_sort bv2.binder_sort;
   faithful_lemma_attrs_dec b1 b2 bv1.binder_attrs bv2.binder_attrs;
   assert_norm (
-      (binding_bv_eq bv1.binder_bv bv2.binder_bv
-       &&& term_eq bv1.binder_sort bv2.binder_sort
-       &&& aqual_eq bv1.binder_qual bv2.binder_qual
-       &&& list_dec_eq b1 b2 term_eq bv1.binder_attrs bv2.binder_attrs) == binder_eq b1 b2);
+      (binding_bv_cmp bv1.binder_bv bv2.binder_bv
+       &&& term_cmp bv1.binder_sort bv2.binder_sort
+       &&& aqual_cmp bv1.binder_qual bv2.binder_qual
+       &&& list_dec_cmp b1 b2 term_cmp bv1.binder_attrs bv2.binder_attrs) == binder_cmp b1 b2);
   ()
 
-and faithful_lemma_qual (q1 q2 : aqualv) : Lemma (requires faithful_qual q1 /\ faithful_qual q2) (ensures defined (aqual_eq q1 q2)) =
+and faithful_lemma_qual (q1 q2 : aqualv) : Lemma (requires faithful_qual q1 /\ faithful_qual q2) (ensures defined (aqual_cmp q1 q2)) =
   match q1, q2 with
   | Q_Meta t1, Q_Meta t2 -> faithful_lemma t1 t2
   | _ -> ()
@@ -749,21 +762,21 @@ and faithful_lemma_attrs_dec #b (top1 top2 : b)
   (at1 : list term{at1 << top1})
   (at2 : list term{at2 << top2})
   : Lemma (requires faithful_attrs at1 /\ faithful_attrs at2)
-          (ensures defined (list_dec_eq top1 top2 term_eq at1 at2))
+          (ensures defined (list_dec_cmp top1 top2 term_cmp at1 at2))
           (decreases at1)
   =
   // TODO: factor out
-  introduce forall x y. L.memP x at1 /\ L.memP y at2 ==> defined (term_eq x y) with
-   (introduce forall y. L.memP x at1 /\ L.memP y at2 ==> defined (term_eq x y) with
-    (introduce (L.memP x at1 /\ L.memP y at2) ==> (defined (term_eq x y)) with h. (
+  introduce forall x y. L.memP x at1 /\ L.memP y at2 ==> defined (term_cmp x y) with
+   (introduce forall y. L.memP x at1 /\ L.memP y at2 ==> defined (term_cmp x y) with
+    (introduce (L.memP x at1 /\ L.memP y at2) ==> (defined (term_cmp x y)) with h. (
      faithful_lemma x y
      )
     )
    )
   ;
-  defined_list_dec top1 top2 term_eq at1 at2
+  defined_list_dec top1 top2 term_cmp at1 at2
 
-and faithful_lemma_comp (c1 c2 : comp) : Lemma (requires faithful_comp c1 /\ faithful_comp c2) (ensures defined (comp_eq c1 c2)) =
+and faithful_lemma_comp (c1 c2 : comp) : Lemma (requires faithful_comp c1 /\ faithful_comp c2) (ensures defined (comp_cmp c1 c2)) =
   match inspect_comp c1, inspect_comp c2 with
   | C_Total t1, C_Total t2 -> faithful_lemma t1 t2
   | C_GTotal t1, C_GTotal t2 -> faithful_lemma t1 t2
@@ -774,32 +787,41 @@ and faithful_lemma_comp (c1 c2 : comp) : Lemma (requires faithful_comp c1 /\ fai
   | C_Eff us1 e1 r1 args1 dec1, C_Eff us2 e2 r2 args2 dec2 ->
     univ_faithful_lemma_list c1 c2 us1 us2;
     faithful_lemma r1 r2;
-    introduce forall x y. L.memP x args1 /\ L.memP y args2 ==> defined (arg_eq x y) with
-     (introduce forall y. L.memP x args1 /\ L.memP y args2 ==> defined (arg_eq x y) with
-      (introduce (L.memP x args1 /\ L.memP y args2) ==> (defined (arg_eq x y)) with h. (
+    introduce forall x y. L.memP x args1 /\ L.memP y args2 ==> defined (arg_cmp x y) with
+     (introduce forall y. L.memP x args1 /\ L.memP y args2 ==> defined (arg_cmp x y) with
+      (introduce (L.memP x args1 /\ L.memP y args2) ==> (defined (arg_cmp x y)) with h. (
        faithful_lemma_arg x y
        )
       )
      )
     ;
-    defined_list_dec c1 c2 arg_eq args1 args2;
-    introduce forall x y. L.memP x dec1 /\ L.memP y dec2 ==> defined (term_eq x y) with
-     (introduce forall y. L.memP x dec1 /\ L.memP y dec2 ==> defined (term_eq x y) with
-      (introduce (L.memP x dec1 /\ L.memP y dec2) ==> (defined (term_eq x y)) with h. (
+    defined_list_dec c1 c2 arg_cmp args1 args2;
+    introduce forall x y. L.memP x dec1 /\ L.memP y dec2 ==> defined (term_cmp x y) with
+     (introduce forall y. L.memP x dec1 /\ L.memP y dec2 ==> defined (term_cmp x y) with
+      (introduce (L.memP x dec1 /\ L.memP y dec2) ==> (defined (term_cmp x y)) with h. (
        faithful_lemma x y
        )
       )
      )
     ;
-    defined_list_dec c1 c2 term_eq dec1 dec2;
+    defined_list_dec c1 c2 term_cmp dec1 dec2;
     (***)comp_eq_C_Eff c1 c2 us1 us2 e1 e2 r1 r2 args1 args2 dec1 dec2;
     ()
   | _ -> ()
 #pop-options
 
+(* A conservative version: works on all terms, returns `true` if they
+are guaranteed to be equal. *)
+let term_eq (t1 t2 : term) : (b:bool{b ==> t1 == t2}) =
+  match term_cmp t1 t2 with
+  | Eq -> true
+  | _ -> false
+
 let faithful_term = t:term{faithful t}
+
+(* A fully decidable version, for faithful terms. *)
 let term_eq_dec (t1 t2 : faithful_term) : (b:bool{b <==> t1 == t2}) =
   faithful_lemma t1 t2;
-  match term_eq t1 t2 with
+  match term_cmp t1 t2 with
   | Eq -> true
   | Neq -> false
